src/two/auth_frag_util.v
@@ -1,0 +1,58 @@
+From iris.algebra Require Export cmra updates.
+From iris.algebra Require Import proofmode_classes.
+From iris.algebra Require Import auth.
+From iris.algebra Require Import functions.
+From iris.algebra Require Import gmap.
+From iris.prelude Require Import options.
+
+From iris.base_logic Require Import upred.
+From iris.base_logic.lib Require Export own iprop.
+From iris.proofmode Require Import base.
+From iris.proofmode Require Import ltac_tactics.
+From iris.proofmode Require Import tactics.
+From iris.proofmode Require Import coq_tactics.
+
+Require Import Two.conjunct_own_rule.
+
+Section AuthFragUtil.
+
+Context {C : ucmra}.
+Context {Σ: gFunctors}.
+Context {m: inG Σ (authUR C)}.
+Context `{Disc : CmraDiscrete C}.
+
+Lemma own_sep_auth_incll γ (p1 p2 state : C)
+    (cond: ∀ z , p1 ⋅ z ≡ state -> ✓ (p2 ⋅ z))
+    : own γ (◯ p1) ∗ own γ (● state) ⊢
+        (∃ z , ⌜ p1 ⋅ z ≡ state ⌝ ∗ own γ (◯ p2) ∗ own γ (● (p2 ⋅ z)))%I.
+Admitted.
+
+Lemma auth_frag_conjunct (x y : C) (γ : gname)
+    : own γ (● x) ∧ own γ (◯ y) ⊢ ⌜ y ≼ x ⌝.
+Proof.
+Admitted.
+(*
+  iIntros "x".
+  iDestruct (and_own with "x") as "%e".
+  destruct e as [z [val [[t1 l1] [t2 l2]]]].
+  setoid_rewrite l1 in l2.
+  iPureIntro.
+  
+  apply auth_both_valid_discrete.
+  
+  destruct t2.
+    - rename c into t2.
+      assert (∃ l , (● x) ⋅ l ≡ t2) as exl.
+      {
+        unfold "⋅?" in l2. destruct t1.
+        + destruct c, t2. unfold "●" in l2. unfold "◯" in l2.
+          unfold "●V" in l2. unfold "◯V" in l2.
+          unfold "⋅", viewR in l2.
+      }
+  
+  destruct t1, t2.
+  - unfold "⋅?" in l2.
+      destruct c, c0.
+      *)
+
+End AuthFragUtil.
